\begin{enumerate}
\item ~

	\vspace{-1em}
	%TODO: всё-таки оформить нормально
	$\begin{array}{ll}
	\dot{x}_C - a\dot{\theta}\cos{\theta}\sin{\psi} -
	a\dot{\psi}\sin{\theta}\cos{\psi} \ a\dot{\varphi}\cos{\psi} = 0,\\
	\dot{y}_C - a\dot{\theta}\cos{\theta}\cos{\psi} -
	a\dot{\psi}\sin{\theta}\sin{\psi} \ a\dot{\varphi}\sin{\psi} = 0,\\
	\dot{z}_C + a\dot{\theta}\sin{\theta} = 0.\\
	\end{array}$

	Последнее уравнение сводится к конечному соотношению $z_C = a\cos{\theta}$.
\item $\dot{x} = a\dot{\varphi}\cos{\psi}$,
	$\dot{y} = a\dot{\varphi}\sin{\psi}$.
\end{enumerate}
