$$ (b-\lambda)x^2+(a-\lambda)y^2=(a-\lambda)(b-\lambda),   \lambda\le a.$$


$$
\dfrac{\pi \lambda}{\sin \pi \lambda} &\quad \text{for $0\leqslant \lambda <\dfrac{1}{2}$,}\\
$$

$$ (b-\lambda)x^2+(a-\lambda)y^2=(a-\lambda)(b-\lambda),   \lambda\ge a.$$


$$
\dfrac{\pi \lambda}{\sin \pi \lambda} &\quad \text{for $0\geq \lambda <\dfrac{1}{2}$,}\\
$$


$$
\dfrac{\pi \lambda}{\sin \pi \lambda} &\quad \text{for $0\leq \lambda <\dfrac{1}{2}$,}\\
$$

$$
\dfrac{\pi \lambda}{\sin \pi \lambda} &\quad \text{for $0\ge \lambda <\dfrac{1}{2}$,}\\
$$

$$
\dfrac{\pi \lambda}{\sin \pi \lambda} &\quad \text{for $0\le \lambda <\dfrac{1}{2}$,}\\
$$
